proof/security/H_MLWE.ec
@@ -3,65 +3,81 @@ require (****) ROM KyberAlgebra.
 
 clone include  KyberAlgebra.
 import Matrix_.
-
-type seed.
-
-op H : seed -> matrix.
-
 abbrev [-printing] m_transpose = trmx.
 
+(* --------------------------------------------------------------------------- *)
+type seed.
+op H : seed -> matrix.
+
+(* --------------------------------------------------------------------------- *)
 op [lossless] dseed : seed distr.
-(* axiom dseed_ll : is_lossless dseed. *)
+(* this automatically add the axiom dseed_ll : is_lossless dseed. *)
+hint solve 0 random : dseed_ll.
 
-(* Uniform distribution over the finite field R *)
+(* --------------------------------------------------------------------------- *)
+(* Uniform distribution over R *)
 op [lossless uniform full] duni_R : R distr.
+(* add duni_R_ll, duni_R_uni, duni_R_fu *)
+(* FIXME: without adding the hint explicitely the hint are lost after cloning *)
+hint solve 0 random : duni_R_ll duni_R_uni duni_R_fu.
 
-op pe : real = mu1 duni_R witness.
-
-lemma duni_R_funi: is_funiform duni_R.
+lemma duni_R_funi : is_funiform duni_R.
 proof. apply is_full_funiform; [apply duni_R_fu | apply duni_R_uni]. qed.
 
-lemma duni_RE: forall (s: R), mu1 duni_R s = pe.
-proof. move=> *; apply duni_R_funi. qed.
-
-(* Distribution over R ( short value ) *)
+(* --------------------------------------------------------------------------- *)
+(* Distribution over R (short values) *)
 
 op [lossless] dshort_R  : R distr.
+hint solve 0 random : dshort_R_ll.
+(* add dshort_R_ll *)
 
-(* We define the distribution over vector *)
+(* --------------------------------------------------------------------------- *)
+(* Extention of those definitions to vector *) 
 op duni = dvector duni_R.
 op dshort = dvector dshort_R.
 
+lemma duni_ll : is_lossless duni.
+proof. apply/dvector_ll/duni_R_ll. qed.
 
-(* FIXME clean the remaining part *)
-op pv : real. 
+lemma duni_fu : is_full duni.
+proof. apply /dvector_full/duni_R_fu. qed.
 
-lemma duni_ll : is_lossless duni by rewrite /duni /dvector; smt.
-axiom duni_vectorE: forall (v: vector), mu1 duni v = pv.
-(* FIXME rename this lemma *)
-lemma duni_vector_uni: is_funiform duni.
-proof. by move=> ??;rewrite !duni_vectorE. qed.
+lemma duni_uni : is_uniform duni.
+proof. apply /dvector_uni/duni_R_uni. qed.
 
-lemma dshort_ll : is_lossless dshort by rewrite /dshort /dvector => />;smt.
+lemma duni_funi : is_funiform duni.
+proof. apply /is_full_funiform; [apply duni_fu | apply duni_uni]. qed.
 
-hint solve 0 random : dshor_ll duni_ll duni_vector_uni.
+hint solve 0 random : duni_ll duni_fu duni_uni duni_funi.
+
+lemma dshort_ll : is_lossless dshort.
+proof. apply/dvector_ll/dshort_R_ll. qed.
+
+hint solve 0 random : dshort_ll.
+
+(* --------------------------------------------------------------------------- *)
+(* Extention of those definitions to matrix *) 
 
 op duni_matrix = dmatrix duni_R.
 
-lemma duni_matrix_ll : is_lossless duni_matrix 
-     by rewrite /duni_matrix /dmatrix => />; smt.
+lemma duni_matrix_ll : is_lossless duni_matrix.
+proof. apply/dmatrix_ll/duni_R_ll. qed.
 
-op pm : real.
-axiom duni_matrixE: forall (m: matrix), mu1 duni_matrix m = pm.
-lemma duni_matrix_uni: is_funiform duni_matrix.
-proof. by move=> ??;rewrite !duni_matrixE. qed.
+lemma duni_matrix_fu : is_full duni_matrix.
+proof. apply /dmatrix_full/duni_R_fu. qed.
 
-op dsample(sd : seed) = duni_matrix.
+lemma duni_matrix_uni : is_uniform duni_matrix.
+proof. apply /dmatrix_uni/duni_R_uni. qed.
+
+lemma duni_matrix_funi : is_funiform duni_matrix.
+proof. apply /is_full_funiform; [apply duni_matrix_fu | apply duni_matrix_uni]. qed.
+
+hint solve 0 random : duni_matrix_ll duni_matrix_fu duni_matrix_uni duni_matrix_funi.
 
 clone import ROM as H_MLWE_ROM with
   type in_t  <- seed,
   type out_t <- matrix,
-  op dout    <- dsample,
+  op dout    <- fun (sd : seed) => duni_matrix, 
   type d_in_t <- unit,
   type d_out_t <- bool.
 import Lazy.
@@ -72,23 +88,24 @@ module type Adv_T = {
 
 module H_MLWE(Adv : Adv_T) = {
 
-   proc main(tr b : bool) : bool = {
-      var sd, s, e, _A, u0, u1, t, e', v0, v1, b';
-
-      sd <$ dseed;
-      s <$ dshort;
-      e <$ dshort;
-      _A <- if tr then m_transpose (H sd) else H sd;
-      u0 <- _A *^ s + e;
-      u1 <$ duni;
-
-      t <$ duni;
-      e' <$ dshort_R;
-      v0 <- (t `<*>` s) +& e';
-      v1 <$ duni_R;
-      
-      b' <@ Adv.guess(sd, t, if b then (u1,v1) else (u0,v0));
-      return b';
+  proc main(tr b : bool) : bool = {
+    var sd, s, e, _A, u0, u1, t, e', v0, v1, b';
+    
+    sd <$ dseed;
+    s <$ dshort;
+    e <$ dshort;
+    _A <- if tr then m_transpose (H sd) else H sd;
+    u0 <- _A *^ s + e;
+    u1 <$ duni;
+    
+    t <$ duni;
+    e' <$ dshort_R;
+    v0 <- (t `<*>` s) +& e';
+    v1 <$ duni_R;
+    
+    b' <@ Adv.guess(sd, t, if b then (u1,v1) else (u0,v0));
+    return b';
    }
+
 }.
 
